src/arch/x64/interop/Vale_poly.fst
@@ -16,8 +16,8 @@ val va_lemma_poly : va_b0:va_code -> va_s0:va_state -> ctx_b:buffer64 -> inp_b:b
   (requires ((va_require_total va_b0 (va_code_poly ()) va_s0) /\ (va_get_ok va_s0) /\ (let
     ctx_in = (va_get_reg Rdi va_s0) in let inp_in = (va_get_reg Rsi va_s0) in let len_in = (va_get_reg Rdx va_s0) in let n = 18446744073709551616 in let p = n
     `op_Multiply` n `op_Multiply` 4 - 5 in len == len_in /\ (buffers_disjoint ctx_b inp_b) /\ (validSrcAddrs64
-    (va_get_mem va_s0) ctx_in ctx_b 24) /\ (validSrcAddrs64 (va_get_mem va_s0) inp_in inp_b
-    (readable_words len_in)) /\ inp_in + len_in < pow2_64)))
+    (va_get_mem va_s0) ctx_in ctx_b 24 (va_get_memTaint va_s0) Public) /\ (validSrcAddrs64 (va_get_mem va_s0) inp_in inp_b
+    (readable_words len_in) (va_get_memTaint va_s0) Public) /\ inp_in + len_in < pow2_64)))
   (ensures (fun (va_sM, va_fM) -> ((va_ensure_total va_b0 va_s0 va_sM va_fM) /\ 
     (va_get_ok va_sM) /\
     (let ctx_in = (va_get_reg Rdi va_s0) in 
@@ -33,7 +33,7 @@ val va_lemma_poly : va_b0:va_code -> va_s0:va_state -> ctx_b:buffer64 -> inp_b:b
     let key_s = (lowerUpper128_opaque key_s0 key_s1) in
     
     (validSrcAddrs64 (va_get_mem va_sM) ctx_in
-    ctx_b 24) /\ (validSrcAddrs64 (va_get_mem va_sM) inp_in inp_b (readable_words len_in)) /\
+    ctx_b 24 (va_get_memTaint va_sM) Public) /\ (validSrcAddrs64 (va_get_mem va_sM) inp_in inp_b (readable_words len_in) (va_get_memTaint va_sM) Public) /\
     (modifies_buffer ctx_b (va_get_mem va_s0) (va_get_mem va_sM)) /\ (let h0_out = (buffer64_read
     ctx_b 0 (va_get_mem va_sM)) in let h1_out = (buffer64_read ctx_b 1 (va_get_mem va_sM)) in
     let h = (lowerUpper128_opaque h0_out h1_out) in (let inp_mem = (seqTo128 (buffer64_as_seq (va_get_mem
@@ -42,12 +42,12 @@ val va_lemma_poly : va_b0:va_code -> va_s0:va_state -> ctx_b:buffer64 -> inp_b:b
     va_sM) == (va_get_reg Rdi va_s0) /\ (va_get_reg Rsi va_sM) == (va_get_reg Rsi va_s0) /\
     (va_get_reg R12 va_sM) == (va_get_reg R12 va_s0) /\ (va_get_reg R13 va_sM) == (va_get_reg R13
     va_s0) /\ (va_get_reg R14 va_sM) == (va_get_reg R14 va_s0) /\ (va_get_reg R15 va_sM) ==
-    (va_get_reg R15 va_s0)))) /\ (va_state_eq va_sM (va_update_mem va_sM (va_update_flags va_sM
+    (va_get_reg R15 va_s0)))) /\ (va_state_eq va_sM (va_update_trace va_sM (va_update_mem va_sM (va_update_flags va_sM
     (va_update_reg Rbp va_sM (va_update_reg Rbx va_sM (va_update_reg R14 va_sM (va_update_reg R12
     va_sM (va_update_reg R11 va_sM (va_update_reg Rdx va_sM (va_update_reg Rsi va_sM (va_update_reg
     Rdi va_sM (va_update_reg R15 va_sM (va_update_reg R13 va_sM (va_update_reg R10 va_sM
     (va_update_reg R9 va_sM (va_update_reg R8 va_sM (va_update_reg Rcx va_sM (va_update_reg Rax
-    va_sM (va_update_ok va_sM va_s0))))))))))))))))))))))
+    va_sM (va_update_ok va_sM va_s0)))))))))))))))))))))))
 
 let va_lemma_poly va_b0 va_s0 ctx_b inp_b len =
   let key_r0 = buffer64_read ctx_b 3 (va_get_mem va_s0) in
